dead end?

NLustreToSyBloc/Correctness.v
@@ -35,21 +35,21 @@ Module Type CORRECTNESS
        (Import Mem   : MEMORIES    Ids Op       Clks SynNL)
        (Import Trans : TRANSLATION Ids Op       Clks SynNL SynSB Mem).
 
-  (* Fixpoint memvar_lexp (x: ident) (e: SynSB.lexp) := *)
-  (*   match e with *)
-  (*   | SynSB.Emem y _ => x = y *)
-  (*   | SynSB.Ewhen e _ _ => memvar_lexp x e *)
-  (*   | SynSB.Eunop _ e _ => memvar_lexp x e *)
-  (*   | SynSB.Ebinop _ e1 e2 _ => memvar_lexp x e1 \/ memvar_lexp x e2 *)
-  (*   | _ => False *)
-  (*   end. *)
+  Fixpoint memvar_lexp (x: ident) (e: SynSB.lexp) :=
+    match e with
+    | SynSB.Ereg y _ => x = y
+    | SynSB.Ewhen e _ _ => memvar_lexp x e
+    | SynSB.Eunop _ e _ => memvar_lexp x e
+    | SynSB.Ebinop _ e1 e2 _ => memvar_lexp x e1 \/ memvar_lexp x e2
+    | _ => False
+    end.
 
-  (* Fixpoint memvar_cexp (x: ident) (ce: SynSB.cexp) := *)
-  (*   match ce with *)
-  (*   | SynSB.Emerge _ e1 e2 => memvar_cexp x e1 \/ memvar_cexp x e2 *)
-  (*   | SynSB.Eite e t f => memvar_lexp x e \/ memvar_cexp x t \/ memvar_cexp x f *)
-  (*   | SynSB.Eexp e => memvar_lexp x e *)
-  (*   end. *)
+  Fixpoint memvar_cexp (x: ident) (ce: SynSB.cexp) :=
+    match ce with
+    | SynSB.Emerge _ e1 e2 => memvar_cexp x e1 \/ memvar_cexp x e2
+    | SynSB.Eite e t f => memvar_lexp x e \/ memvar_cexp x t \/ memvar_cexp x f
+    | SynSB.Eexp e => memvar_lexp x e
+    end.
 
   Definition memory_spec (m: SemSB.memory) (memids: PS.t) (R: env) :=
     forall x v,
@@ -139,57 +139,87 @@ Module Type CORRECTNESS
         induction 1; simpl; eauto using SemSB.sem_cexp_instant.
       Qed.
 
-      (* Lemma sem_lexp_instant_madd_mem: *)
-      (*   forall x mv e v, *)
-      (*     SemSB.sem_lexp_instant base R m e v -> *)
-      (*     ~ memvar_lexp x e -> *)
-      (*     SemSB.sem_lexp_instant base R (madd_mem x mv m) e v. *)
-      (* Proof. *)
-      (*   induction 1; simpl; intros Nmv; eauto using SemSB.sem_lexp_instant. *)
-      (*   - do 2 constructor. *)
-      (*     match goal with H: SemSB.sem_mem_var_instant _ _ _ |- _ => inv H end. *)
-      (*     unfold SemSB.get_mem in *. *)
-      (*     rewrite mfind_mem_gso; auto. *)
-      (*   - econstructor; eauto. *)
-      (*   - econstructor; eauto. *)
-      (* Qed. *)
-      (* Hint Resolve sem_lexp_instant_madd_mem. *)
+      Lemma sem_lexp_instant_madd_mem:
+        forall x mv e v,
+          SemSB.sem_lexp_instant base R m e v ->
+          ~ memvar_lexp x e ->
+          SemSB.sem_lexp_instant base R (madd_mem x mv m) e v.
+      Proof.
+        induction 1; simpl; intros; eauto using SemSB.sem_lexp_instant.
+        - do 2 constructor.
+          match goal with H: SemSB.sem_mem_var_instant _ _ _ |- _ => inv H end.
+          unfold SemSB.get_reg in *.
+          rewrite mfind_mem_gso; auto.
+        - econstructor; eauto.
+        - econstructor; eauto.
+      Qed.
+      Hint Resolve sem_lexp_instant_madd_mem.
 
-      (* Lemma sem_cexp_instant_madd_mem: *)
-      (*   forall x mv ce v, *)
-      (*     SemSB.sem_cexp_instant base R m ce v -> *)
-      (*     ~ memvar_cexp x ce -> *)
-      (*     SemSB.sem_cexp_instant base R (madd_mem x mv m) ce v. *)
-      (* Proof. *)
-      (*   induction 1; simpl; intros Nmv; eauto using SemSB.sem_cexp_instant. *)
-      (*   - econstructor; eauto. *)
-      (*   - econstructor 2; eauto. *)
-      (*   - econstructor; eauto. *)
-      (*   - econstructor; eauto. *)
-      (*     + apply IHsem_cexp_instant1; auto. *)
-      (*     + apply IHsem_cexp_instant2; auto. *)
-      (*   - econstructor; eauto. *)
-      (*     + apply IHsem_cexp_instant1; auto. *)
-      (*     + apply IHsem_cexp_instant2; auto. *)
-      (* Qed. *)
+      Lemma sem_cexp_instant_madd_mem:
+        forall x mv ce v,
+          SemSB.sem_cexp_instant base R m ce v ->
+          ~ memvar_cexp x ce ->
+          SemSB.sem_cexp_instant base R (madd_mem x mv m) ce v.
+      Proof.
+        induction 1; simpl; intros; eauto using SemSB.sem_cexp_instant.
+        - econstructor; eauto.
+        - econstructor 2; eauto.
+        - econstructor; eauto.
+        - econstructor; eauto.
+          + apply IHsem_cexp_instant1; auto.
+          + apply IHsem_cexp_instant2; auto.
+        - econstructor; eauto.
+          + apply IHsem_cexp_instant1; auto.
+          + apply IHsem_cexp_instant2; auto.
+      Qed.
 
-      (* Lemma sem_lexps_instant_madd_mem: *)
-      (*   forall x mv es vs, *)
-      (*     SemSB.sem_lexps_instant base R m es vs -> *)
-      (*     Forall (fun e => ~ memvar_lexp x e) es -> *)
-      (*     SemSB.sem_lexps_instant base R (madd_mem x mv m) es vs. *)
-      (* Proof. *)
-      (*   induction 1; simpl; intros Nmv; inv Nmv. *)
-      (*   - constructor. *)
-      (*   - constructor; auto. *)
-      (*     apply IHForall2; auto. *)
-      (* Qed. *)
+      Lemma sem_lexps_instant_madd_mem:
+        forall x mv es vs,
+          SemSB.sem_lexps_instant base R m es vs ->
+          Forall (fun e => ~ memvar_lexp x e) es ->
+          SemSB.sem_lexps_instant base R (madd_mem x mv m) es vs.
+      Proof.
+        induction 1; simpl; intros Nmv; inv Nmv.
+        - constructor.
+        - constructor; auto.
+          apply IHForall2; auto.
+      Qed.
+
+      Lemma sem_lexp_instant_madd_obj:
+        forall x m' e v,
+          SemSB.sem_lexp_instant base R m e v ->
+          SemSB.sem_lexp_instant base R (madd_obj x m' m) e v.
+      Proof.
+        induction 1; simpl; intros; eauto using SemSB.sem_lexp_instant.
+        do 2 constructor.
+        match goal with H: SemSB.sem_mem_var_instant _ _ _ |- _ => inv H end.
+        unfold SemSB.get_reg in *.
+        now rewrite mfind_mem_add_inst.
+      Qed.
+      Hint Resolve sem_lexp_instant_madd_obj.
+
+      Lemma sem_cexp_instant_madd_obj:
+        forall x m' ce v,
+          SemSB.sem_cexp_instant base R m ce v ->
+          SemSB.sem_cexp_instant base R (madd_obj x m' m) ce v.
+      Proof.
+        induction 1; simpl; intros; eauto using SemSB.sem_cexp_instant.
+      Qed.
+
+      Lemma sem_lexps_instant_madd_obj:
+        forall x m' es vs,
+          SemSB.sem_lexps_instant base R m es vs ->
+          SemSB.sem_lexps_instant base R (madd_obj x m' m) es vs.
+      Proof.
+        induction 1; simpl; intros; constructor; auto.
+      Qed.
 
     End SemInstant.
     Hint Resolve var_instant_correctness clock_instant_correctness
          lexp_instant_correctness lexps_instant_correctness
-         cexp_instant_correctness.
-         (* sem_cexp_instant_madd_mem sem_lexps_instant_madd_mem. *)
+         cexp_instant_correctness
+         sem_cexp_instant_madd_mem sem_lexps_instant_madd_mem
+         sem_cexp_instant_madd_obj sem_lexps_instant_madd_obj.
 
     Lemma pm_map_add:
       forall {A B} (m: PM.t A) (f: A -> B) x v,
@@ -207,6 +237,18 @@ Module Type CORRECTNESS
       f_equal.
       - now rewrite pm_map_add, mm_values_map.
       - now rewrite mm_instances_map.
+    Qed.
+
+    Lemma restr_mem_madd_obj:
+      forall x M' M n,
+        SemSB.restr_mem (madd_obj x M' M) n =
+        madd_obj x (SemSB.restr_mem M' n) (SemSB.restr_mem M n).
+    Proof.
+      intros.
+      unfold SemSB.restr_mem, madd_obj; simpl.
+      f_equal.
+      - now rewrite mm_values_map.
+      - now rewrite pm_map_add, mm_instances_map.
     Qed.
 
     Section Sem.
@@ -278,36 +320,61 @@ Module Type CORRECTNESS
         - induction Sem; repeat constructor; auto.
       Qed.
 
-      (* Lemma sem_caexp_madd_mem: *)
-      (*   forall x mvs ck ce xs, *)
-      (*     SemSB.sem_caexp bk H M ck ce xs -> *)
-      (*     ~ memvar_cexp x ce -> *)
-      (*     SemSB.sem_caexp bk H (madd_mem x mvs M) ck ce xs. *)
-      (* Proof. *)
-      (*   intros ** Sem ? n; specialize (Sem n); inv Sem; *)
-      (*     econstructor; eauto; *)
-      (*       rewrite restr_mem_madd_mem; auto. *)
-      (* Qed. *)
+      Lemma sem_caexp_madd_mem:
+        forall x mvs ck ce xs,
+          SemSB.sem_caexp bk H M ck ce xs ->
+          ~ memvar_cexp x ce ->
+          SemSB.sem_caexp bk H (madd_mem x mvs M) ck ce xs.
+      Proof.
+        intros ** Sem ? n; specialize (Sem n); inv Sem;
+          econstructor; eauto;
+            rewrite restr_mem_madd_mem; auto.
+      Qed.
 
-      (* Lemma sem_laexps_madd_mem: *)
-      (*   forall x mvs ck es xss, *)
-      (*     SemSB.sem_laexps bk H M ck es xss -> *)
-      (*     Forall (fun e => ~ memvar_lexp x e) es -> *)
-      (*     SemSB.sem_laexps bk H (madd_mem x mvs M) ck es xss. *)
-      (* Proof. *)
-      (*   intros ** Sem ? n; specialize (Sem n); inv Sem. *)
-      (*   - econstructor; eauto. *)
-      (*     rewrite restr_mem_madd_mem; auto. *)
-      (*   - econstructor 2; eauto. *)
-      (*     rewrite restr_mem_madd_mem; auto. *)
-      (*   - constructor 3. *)
-      (* Qed. *)
+      Lemma sem_laexps_madd_mem:
+        forall x mvs ck es xss,
+          SemSB.sem_laexps bk H M ck es xss ->
+          Forall (fun e => ~ memvar_lexp x e) es ->
+          SemSB.sem_laexps bk H (madd_mem x mvs M) ck es xss.
+      Proof.
+        intros ** Sem ? n; specialize (Sem n); inv Sem.
+        - econstructor; eauto.
+          rewrite restr_mem_madd_mem; auto.
+        - econstructor 2; eauto.
+          rewrite restr_mem_madd_mem; auto.
+        - constructor 3.
+      Qed.
+
+      Lemma sem_caexp_madd_obj:
+        forall x M' ck ce xs,
+          SemSB.sem_caexp bk H M ck ce xs ->
+          SemSB.sem_caexp bk H (madd_obj x M' M) ck ce xs.
+      Proof.
+        intros ** Sem n; specialize (Sem n); inv Sem;
+          econstructor; eauto;
+            rewrite restr_mem_madd_obj; auto.
+      Qed.
+      Hint Resolve sem_caexp_madd_obj.
+
+      Lemma sem_laexps_madd_obj:
+        forall x M' ck es xss,
+          SemSB.sem_laexps bk H M ck es xss ->
+          SemSB.sem_laexps bk H (madd_obj x M' M) ck es xss.
+      Proof.
+        intros ** Sem n; specialize (Sem n); inv Sem.
+        - econstructor; eauto.
+          rewrite restr_mem_madd_obj; auto.
+        - econstructor 2; eauto.
+          rewrite restr_mem_madd_obj; auto.
+        - constructor 3.
+      Qed.
+      Hint Resolve sem_laexps_madd_obj.
 
       (* Lemma sem_equation_madd_mem: *)
-      (*   forall x mvs mems k eqs, *)
+      (*   forall x mvs eqs, *)
       (*     (* ~Is_defined_in_eqs x eqs -> *) *)
-      (*     Forall (SemSB.sem_equation P k bk H M mems) eqs -> *)
-      (*     Forall (SemSB.sem_equation P k bk H (madd_mem x mvs M) mems) eqs. *)
+      (*     Forall (SemSB.sem_equation P bk H M) eqs -> *)
+      (*     Forall (SemSB.sem_equation P bk H (madd_mem x mvs M)) eqs. *)
       (* Proof. *)
       (*   intros ** (* Hnd *) Hsem. *)
       (*   induction eqs as [|eq eqs IH]; [now constructor|]. *)
@@ -319,16 +386,126 @@ Module Type CORRECTNESS
       (*   - econstructor; eauto. *)
       (*     apply sem_caexp_madd_mem; auto. *)
       (*     admit. *)
-      (*   - admit. *)
+      (*   - econstructor; eauto. *)
+      (*     apply sem_caexp_madd_mem; eauto. *)
+      (*     admit. *)
+      (*     admit. *)
       (*   - econstructor; eauto. *)
       (*     apply sem_laexps_madd_mem; auto. *)
       (*     admit. *)
       (* Admitted. *)
+      Inductive inst_in_eq: ident -> SynSB.equation -> Prop :=
+      | DefEqReset:
+          forall x ck m r,
+            inst_in_eq x (SynSB.EqReset ck m x r)
+      | DefEqCall:
+          forall x xs ck m es,
+            inst_in_eq x (SynSB.EqCall xs ck m x es).
+
+      Definition inst_in_eqs (x: ident) (eqs: list SynSB.equation) : Prop :=
+        List.Exists (inst_in_eq x) eqs.
+
+      Lemma not_inst_in_eq_cons:
+        forall x eq eqs,
+          ~ inst_in_eqs x (eq :: eqs)
+          <-> ~ inst_in_eq x eq /\ ~ inst_in_eqs x eqs.
+      Proof.
+        split.
+        - intro Hndef; split; intro;
+            eapply Hndef; constructor (assumption).
+        - intros [? ?] Hdef_all.
+          inv Hdef_all; eauto.
+      Qed.
+
+
+
+      Lemma sem_equation_madd_obj:
+        forall M' x eqs,
+          ~ inst_in_eqs x eqs ->
+          Forall (SemSB.sem_equation P bk H M) eqs ->
+          Forall (SemSB.sem_equation P bk H (madd_obj x M' M)) eqs.
+      Proof.
+        intros * Hnd Hsem.
+        induction eqs as [|eq eqs IH]; [now constructor|].
+        apply not_inst_in_eq_cons in Hnd as [Hnd Hnds].
+        apply Forall_cons2 in Hsem as [Hsem Hsems].
+        constructor; auto.
+        induction eq; inv Hsem; eauto using SemSB.sem_equation.
+        - econstructor; eauto.
+          match goal with H: SemSB.next_reg _ _ _ |- _ => inv H end.
+          econstructor; eauto.
+        - econstructor; eauto.
+          unfold sub_inst; rewrite mfind_inst_gso; auto.
+          intro; apply Hnd; subst.
+          constructor.
+        - econstructor; eauto.
+          unfold sub_inst; rewrite mfind_inst_gso; auto.
+          intro; apply Hnd; subst.
+          constructor.
+      Qed.
 
     End Sem.
     Hint Resolve var_correctness vars_correctness
          laexp_correctness caexp_correctness laexps_correctness.
 
+    Fixpoint well_formed_eqs (eqs: list SynSB.equation) : Prop :=
+        match eqs with
+        | [] => True
+        | SynSB.EqReset _ _ x _ :: eqs => ~ inst_in_eqs x eqs /\ well_formed_eqs eqs
+        | SynSB.EqCall _ _ _ x _ :: eqs => ~ inst_in_eqs x eqs /\ well_formed_eqs eqs
+        | _ :: eqs => well_formed_eqs eqs
+        end.
+
+    Lemma memories_spec_madd_obj:
+      forall M memids H x M',
+        memories_spec M memids H ->
+        memories_spec (madd_obj x M' M) memids H.
+    Proof.
+      intros ** Spec n x' v Find Mem.
+      specialize (Spec n x' v Find Mem).
+      unfold SemSB.get_reg in *.
+      now rewrite restr_mem_madd_obj, mfind_mem_add_inst.
+    Qed.
+    Hint Resolve memories_spec_madd_obj.
+
+    Lemma sem_msem_eq:
+      forall bk H eqs M eq memids (* argIn *),
+        (forall f xss oss,
+            sem_node G f xss oss ->
+            exists M, SemSB.sem_block P f M xss oss) ->
+        (forall f r xss oss,
+            sem_reset G f r xss oss ->
+            exists M, SemSB.sem_block P f M xss oss
+                 /\ SemSB.reset_regs r M) ->
+        sem_equation G bk H eq ->
+        memories_spec M memids H ->
+        well_formed_eqs (translate_eqn memids eq ++ eqs) ->
+        (* Is_well_sch mems argIn (eq :: eqs) -> *)
+        Forall (SemSB.sem_equation P bk H M) eqs ->
+        exists M', Forall (SemSB.sem_equation P bk H M') (translate_eqn memids eq ++ eqs).
+    Proof.
+      intros ** IHnode IHreset Heq Spec WF Heqs.
+      inv Heq; simpl.
+      - repeat (econstructor; eauto).
+      - edestruct IHnode as (M' & Block); eauto.
+        exists (madd_obj (hd default x) M' M).
+        econstructor; eauto.
+        + econstructor; eauto.
+          apply mfind_inst_gss.
+        + apply sem_equation_madd_obj; auto.
+          apply WF.
+      - edestruct IHreset as (M' & Block & Reset); eauto.
+        exists (madd_obj (hd default x) M' M).
+        econstructor; eauto.
+        + econstructor; eauto.
+          apply mfind_inst_gss.
+        + econstructor; eauto.
+          * econstructor; eauto.
+            apply mfind_inst_gss.
+          * apply sem_equation_madd_obj; auto.
+            apply WF.
+      - exists (madd_mem x {| SynSB.content := hold (sem_const c0) ls; SynSB.reset := fun _ => false |} M).
+          SearchAbout mfind_inst. apply laexps_correctness; auto.
 
     Theorem correctness:
       forall f xss oss,
@@ -386,12 +563,18 @@ Module Type CORRECTNESS
         + apply sem_caexp_laexp; eauto.
         + econstructor.
           * apply mfind_mem_gss.
-          * simpl; intro n.
-            subst. unfold fby. simpl.
-            admit.
+          * simpl; subst; reflexivity.
 
       - admit.
 
-      - admit.
+      - eexists.
+        match goal with
+          H: find_node _ _ = _ |- _ => apply find_node_translate in H as (bl & ? & Find & E)
+        end.
+        subst.
+        econstructor; eauto.
+        + simpl; rewrite map_fst_idty; eauto.
+        + simpl; rewrite map_fst_idty; eauto.
+        + simpl.
 
     Qed.
